Test/SmtTranslation/BoolNatInt.lean
@@ -14,6 +14,8 @@ example : max 3 4 = 4 ∧ min 1 2 = 1 := by auto
 
 example : (2 : Int) = ((nat_lit 2) : Int) := by auto
 
+example : max (-3) 4 = 4 ∧ min 1 (-2) = -2 := by auto
+
 example {α β : Type} (f : α → Nat → β → α → Nat) :
   ∀ a b c, f a 1 b c = f a 1 b c := by auto
 
